feat: enforce max encrypted data keys (#470)

src/SDK/AwsEncryptionSdk.dfy
@@ -52,6 +52,7 @@ module {:extern "Dafny.Aws.Esdk.AwsEncryptionSdkClient"} AwsEncryptionSdk {
         const config: Esdk.AwsEncryptionSdkClientConfig;
 
         const commitmentPolicy: Crypto.CommitmentPolicy;
+        const maxEncryptedDataKeys: Option<int64>;
 
         constructor (config: Esdk.AwsEncryptionSdkClientConfig)
             ensures this.config == config
@@ -62,8 +63,17 @@ module {:extern "Dafny.Aws.Esdk.AwsEncryptionSdkClient"} AwsEncryptionSdk {
 
             ensures config.commitmentPolicy.Some? ==>
                 this.commitmentPolicy == config.commitmentPolicy.value
+
+            ensures this.maxEncryptedDataKeys == config.maxEncryptedDataKeys
         {
             this.config := config;
+
+            // TODO: Ideally we would validate that this value, if provided, falls within a specific range,
+            // then only pass around known good values to all places where it is used.
+            // However, currently Polymorph doesn't handle this smoothly for these service client
+            // constructors and their configurations.
+            this.maxEncryptedDataKeys := config.maxEncryptedDataKeys;
+
             if config.commitmentPolicy.None? {
                 var defaultPolicy := ConfigDefaults.GetDefaultCommitmentPolicy(config.configDefaults);
                 this.commitmentPolicy := defaultPolicy;
@@ -126,6 +136,11 @@ module {:extern "Dafny.Aws.Esdk.AwsEncryptionSdkClient"} AwsEncryptionSdk {
             }
             :- Need(maxPlaintextLength < INT64_MAX_LIMIT, "Input plaintext size too large.");
 
+            // TODO: Change to '> 0' once CrypTool-4350 complete
+            // TODO: Remove entirely once we can validate this value on client creation
+            if this.maxEncryptedDataKeys.Some? {
+                :- Need(this.maxEncryptedDataKeys.value >= 0, "maxEncryptedDataKeys must be non-negative");
+            }
 
             var cmm := input.materialsManager;
             // TODO: bring back once we can have Option<Trait>
@@ -153,6 +168,15 @@ module {:extern "Dafny.Aws.Esdk.AwsEncryptionSdkClient"} AwsEncryptionSdk {
                 input.encryptionContext,
                 maxPlaintextLength as int64
             );
+
+            //= compliance/client-apis/encrypt.txt#2.6.1
+            //# If the number of
+            //# encrypted data keys (../framework/structures.md#encrypted-data-keys)
+            //# on the encryption materials (../framework/structures.md#encryption-
+            //# materials) is greater than the maximum number of encrypted data keys
+            //# (client.md#maximum-number-of-encrypted-data-keys) configured in the
+            //# client (client.md) encrypt MUST yield an error.
+            var _ :- ValidateMaxEncryptedDataKeys(materials.encryptedDataKeys);
 
             //= compliance/client-apis/encrypt.txt#2.6.1
             //# If this
@@ -480,6 +504,12 @@ module {:extern "Dafny.Aws.Esdk.AwsEncryptionSdkClient"} AwsEncryptionSdk {
             //:- Need(request.cmm == null || request.keyring == null, "DecryptRequest.keyring OR DecryptRequest.cmm must be set (not both).");
             //:- Need(request.cmm != null || request.keyring != null, "DecryptRequest.cmm and DecryptRequest.keyring cannot both be null.");
 
+            // TODO: Change to '> 0' once CrypTool-4350 complete
+            // TODO: Remove entirely once we can validate this value on client creation
+            if this.maxEncryptedDataKeys.Some? {
+                :- Need(this.maxEncryptedDataKeys.value >= 0, "maxEncryptedDataKeys must be non-negative");
+            }
+
             var cmm := input.materialsManager;
             // TODO: bring back once we can have Option<Trait>
             /*
@@ -495,11 +525,10 @@ module {:extern "Dafny.Aws.Esdk.AwsEncryptionSdkClient"} AwsEncryptionSdk {
 
             var buffer := SerializeFunctions.ReadableBuffer(input.ciphertext, 0);
             var headerBody :- Header
-                .ReadHeaderBody(buffer)
+                .ReadHeaderBody(buffer, this.maxEncryptedDataKeys)
                 .MapFailure(EncryptDecryptHelpers.MapSerializeFailure(": ReadHeaderBody"));
 
             var rawHeader := headerBody.tail.bytes[buffer.start..headerBody.tail.start];
-
 
             var algorithmSuiteId := SerializableTypes.GetAlgorithmSuiteId(headerBody.data.esdkSuiteId);
             var _ := Client.SpecificationClient().ValidateCommitmentPolicyOnDecrypt(
@@ -637,6 +666,32 @@ module {:extern "Dafny.Aws.Esdk.AwsEncryptionSdkClient"} AwsEncryptionSdk {
             :- Need(SerializableTypes.IsESDKEncryptionContext(decMat.encryptionContext), "CMM failed to return serializable encryption materials.");
 
             return Success(decMat);
+        }
+
+        method ValidateMaxEncryptedDataKeys(edks: SerializableTypes.ESDKEncryptedDataKeys)
+            returns (res: Result<(), string>)
+
+        // TODO: change to '> 0' once CrypTool-4350 fixed
+        requires this.maxEncryptedDataKeys.Some? ==> this.maxEncryptedDataKeys.value >= 0
+
+        ensures this.maxEncryptedDataKeys.None? ==> res.Success?
+
+        ensures
+            && this.maxEncryptedDataKeys.Some?
+            && this.maxEncryptedDataKeys.value > 0 // TODO: remove once CrypTool-4350 fixed
+            && |edks| as int64 > this.maxEncryptedDataKeys.value
+        ==>
+            res.Failure?
+        {
+            if
+                && this.maxEncryptedDataKeys.Some?
+                && this.maxEncryptedDataKeys.value > 0 // TODO: remove once CrypTool-4350 fixed
+                && |edks| as int64 > this.maxEncryptedDataKeys.value
+            {
+                return Failure("Encrypted data keys exceed maxEncryptedDataKeys");
+            } else {
+                return Success(());
+            }
         }
 
     }
